\documentclass[a4paper]{article}
\usepackage{amsmath}
\usepackage{bm}
\usepackage{xcolor}
\usepackage{braket}
\usepackage{amssymb}
\usepackage{mathrsfs}
\usepackage{mathtools}
\begin{document}
	\title{Chapter\;7}
	\date{ }
	\maketitle
\section{Time order}
Define time order symbol $T[\cdot]$:$$T[A_1(t_1)A_2(t_2)\cdots A_n(t_n)]=A_{j_1}(t_{j_1})A_{j_2}(t_{j_1})\cdots A_{j_n}(t_n)$$
where $$t_{j_1}\geq t_{j_2}\geq\cdots t_{j_n}$$quick mnemonic is 'later on the left'.When there exists $t_{j_k}=t_{j_{k+1}}$,there is ambiguity of ordering of these two terms,but in the problem we're dealing with,these two equal time operator commute so we don't need to worry about it.
\par One must notice that $T[\cdot]$ can only act on single one product.Operations like $T[A-B]$ are invalid.
\section{interaction picture}
Suppose the Hamiltonian of system can be written as$$\hat{H}=\hat{H}_0+\hat{H}_I$$where $\hat{H}_0$ is solvable part and $\hat{H}_I$ is unsolvable part which is usually interaction part.We use subscript S,I to denote quantity in Schrodinger picture and interaction picture respectively,then in interaction picture,we define states and operators as follow:
\begin{align*}
	&\ket{\psi(t)}_I=e^{i\hat{H}_0t}\ket{\psi(t)}_S\\
	&A_I(t)=e^{i\hat{H}_0t}A_S(t)e^{-i\hat{H}_0t}
\end{align*}
Let$$\hat{H}'=e^{i\hat{H}_0t}H_Ie^{-i\hat{H}_0t}$$
which is the interaction part of Hamiltonian in interaction picture.Then we have Schrodinger equation in interaction picture:$$i\frac{d}{dt}\ket{\psi(t)}_I=\hat{H}'\ket{\psi(t)}_I$$
Define time evolution operator in interaction picture to be $\hat{U}_I(t_2,t_1)$ that satisfies $\ket{\psi(t_2)}_I=\hat{U}_I(t_2,t_1)\ket{\psi(t_1)}_I$,then the differential equation for $\hat{U}_I(t,t')$ is$$i\frac{\partial}{\partial t}\hat{U}_I(t,t')=\hat{H}'\hat{U}_I(t,t')$$whose solution is$$\hat{U}_I(t,t')=T[e^{-i\int_{t'}^{t}\hat{H}'(\xi)d\xi}]$$
\section{process of scattering}
In the scattering setting,we shoot wave pack into the potential from far past and recieve wave pack from far future.Let $\hat{H}$ be full Hamiltonian which includes the potential and $\hat{H}_0$ be free Hamiltonian.Solution to full Hamiltonian is a vector in Hilbert space $\mathscr{H}$ and solution to free Hamiltonian is a vector in Hilbert space $\mathscr{H}_0$.
\par In $\mathscr{H}$ there exist solutions in far past and far future looking like vectors $\ket{\psi(t)}$(for far past) and $\ket{\phi(t)}$(for far future) in $\mathscr{H}_0$.Let them be $\ket{\psi(t)}^{in}$ for state that is asymptotically  $\ket{\psi(t)}$ in far past and $\ket{\phi(t)}^{out}$ for state that is asymptotically $\ket{\phi(t)}$ in far future.
\par states in $\mathscr{H}$ evolve according to $\hat{U}_{\hat{H}}(t,t')=e^{-i\hat{H}(t-t')}$ and states in $\mathscr{H}_0$ evolve according to $\hat{U}_{\hat{H}_0}(t,t')=e^{-i\hat{H}_0(t-t')}$.By saying 'asymptotically',it actually means
\begin{align*}
	&\lim_{t\rightarrow -\infty}||\hat{U}_{\hat{H}_0}(t,0)\ket{\psi}-\hat{U}_{\hat{H}}(t,0)\ket{\psi}^{in}||=0\\&\lim_{t\rightarrow -\infty}||\hat{U}_{\hat{H}_0}(t,0)\ket{\phi}-\hat{U}_{\hat{H}}(t,0)\ket{\phi}^{out}||=0
\end{align*}
where we've defined
\begin{align*}
	&\ket{\psi}\equiv\ket{\psi(0)},\ket{\psi}^{in}\equiv\ket{\psi(0)}^{in}\\&\ket{\phi}\equiv\ket{\phi(0)},\ket{\phi}^{out}\equiv\ket{\phi(0)}^{out}
\end{align*}
\section{S-matrix}
We define an extremely important quantity in QFT,called S-matrix:$$\bra{\phi}S\ket{\psi}\equiv\, ^{out}\braket{\phi|\psi}^{in}$$
S-matrix obeys certain properties:
\par (1)$S$ conserves probability,that is $S^{\dagger}S=SS^{\dagger}=1$
\par (2)$S$ comnutes with free energy $\hat{H}_0$.Because,first,$S$ is an operator in $\mathscr{H}_0$,it turns an free state into another who has exactly the same energy,so compute$$[S,\hat{H}_0]\ket{\psi_1}=ES\ket{\psi_1}-\hat{H}_0S\ket{\psi_1}=ES\ket{\psi_1}-ES\ket{\psi_1}=0$$where $E$ is the energy of free state.Thereby we must have $[S,\hat{H}_0]=0$
From these two properties,we can derivate the expression for $S$.We first simplify $ ^{out}\braket{\phi|\psi}^{in}$:
\begin{align*}
	^{out}\braket{\phi|\psi}^{in}&=\braket{^{out}_I\phi|\psi}^{in}_I=\bra{^{out}_I\phi(\infty)}\hat{U}^{\dagger}_I(0,\infty)\hat{U}_I(0,-\infty)\ket{\psi(-\infty)}^{in}_I\\&=\bra{^{out}\phi(\infty)}\hat{U}^{\dagger}_{\hat{H}_0}(0,\infty)\hat{U}^{\dagger}_I(0,\infty)\hat{U}_I(0,-\infty)\hat{U}_{\hat{H}_0}(0,-\infty)\ket{\psi(-\infty)}^{in}\\&=\bra{\phi(\infty)}\hat{U}^{\dagger}_{\hat{H}_0}(0,\infty)\hat{U}^{\dagger}_I(0,\infty)\hat{U}_I(0,-\infty)\hat{U}_{\hat{H}_0}(0,-\infty)\ket{\psi(-\infty)}\\&=\bra{\phi}\hat{U}_I(\infty,-\infty)\ket{\psi}=\bra{\phi}S\ket{\psi}
\end{align*}
Therefore,we find that$$S=\hat{U}_I(\infty,-\infty)=T[e^{-i\int_{t'}^{t}\hat{H}'(\xi)d\xi}]$$
\end{document}